pulse/lib/steel/pulse/Pulse.Checker.WithLocal.fst
@@ -29,7 +29,8 @@ let extend_post_hint_for_local (g:env) (p:post_hint_for_env g)
   : T.Tac (q:post_hint_for_env (push_binding g x ppname_default (mk_ref init_t)){ 
       q.post == comp_withlocal_body_post p.post init_t (null_var x) /\
       q.ret_ty == p.ret_ty /\
-      q.u == p.u
+      q.u == p.u /\
+      q.effect_annot == p.effect_annot
       })
   = let conjunct = tm_exists_sl u0 (as_binder init_t) (mk_pts_to init_t (null_var x) (null_bvar 0)) in
     let g' = push_binding g x ppname_default (mk_ref init_t) in
@@ -45,6 +46,10 @@ let with_local_pre_typing (#g:env) (#pre:term) (pre_typing:tot_typing g pre tm_v
   = admit()
 
 #push-options "--z3rlimit_factor 4 --fuel 0 --ifuel 1"
+let head_range (t:st_term {Tm_WithLocal? t.term}) : range =
+  let Tm_WithLocal { initializer } = t.term in
+  initializer.range
+
 let check
   (g:env)
   (pre:term)
@@ -53,65 +58,72 @@ let check
   (res_ppname:ppname)
   (t:st_term { Tm_WithLocal? t.term })
   (check:check_t)
-  : T.Tac (checker_result_t g pre post_hint) =
+: T.Tac (checker_result_t g pre post_hint)
+= match post_hint with
+  | None ->
+    fail g (Some <| head_range t)
+      "Allocating a mutable local variable expects an annotated post-condition"
 
-  let g = push_context "check_withlocal" t.range g in
-  let Tm_WithLocal {binder; initializer=init; body} = t.term in
-  let (| init, init_u, init_t, init_t_typing, init_typing |) =
-    (* Check against annotation if any *)
-    let ty = binder.binder_ty in
-    match ty.t with
-    | Tm_Unknown -> compute_tot_term_type_and_u g init
-    | _ ->
-      let (| u, ty_typing |) = check_universe g ty in
-      let (| init, init_typing |) = check_term g init T.E_Total ty in
-      let ty_typing : universe_of g ty u = ty_typing in
-      let init_typing : typing g init T.E_Total ty = init_typing in
-      (| init, u, ty, ty_typing, init_typing |)
-        <: (t:term & u:universe & ty:term & universe_of g ty u & tot_typing g t ty)
-        (* ^ Need this annotation *)
-    in
-  if eq_univ init_u u0
-  then
-    let x = fresh g in
-    let px = binder.binder_ppname, x in
-    if x `Set.mem` freevars_st body
-    then fail g (Some body.range) (Printf.sprintf "withlocal: %s is free in body" (T.unseal binder.binder_ppname.name))
-    else
-      let x_tm = term_of_nvar px in
-      let g_extended = push_binding g x binder.binder_ppname (mk_ref init_t) in
-      let body_pre = comp_withlocal_body_pre pre init_t x_tm init in
-      let body_pre_typing = with_local_pre_typing pre_typing init_t x init in
-      // elaborating this post here,
-      //   so that later we can check the computed post to be equal to this one
-      let post : post_hint_for_env g =
-        match post_hint with
-        | Some post -> post
-        | None -> fail g None "Allocating a mutable local variable expects an annotated post-condition"
+  | Some { effect_annot = EffectAnnotGhost }
+  | Some { effect_annot = EffectAnnotAtomic _ } ->
+    fail g (Some <| head_range t)
+      "Allocating a mutable local variable is only allowed in non-ghost and non-atomic code"
+
+  | Some post ->
+    let g = push_context "check_withlocal" t.range g in
+    let Tm_WithLocal {binder; initializer=init; body} = t.term in
+    let (| init, init_u, init_t, init_t_typing, init_typing |) =
+      (* Check against annotation if any *)
+      let ty = binder.binder_ty in
+      match ty.t with
+      | Tm_Unknown -> compute_tot_term_type_and_u g init
+      | _ ->
+        let (| u, ty_typing |) = check_universe g ty in
+        let (| init, init_typing |) = check_term g init T.E_Total ty in
+        let ty_typing : universe_of g ty u = ty_typing in
+        let init_typing : typing g init T.E_Total ty = init_typing in
+        (| init, u, ty, ty_typing, init_typing |)
+          <: (t:term & u:universe & ty:term & universe_of g ty u & tot_typing g t ty)
+          (* ^ Need this annotation *)
       in
-      if x `Set.mem` freevars post.post
-      then fail g None "Impossible! check_withlocal: unexpected name clash in with_local,\
-                        please file a bug-report"
+    if not (eq_univ init_u u0)
+    then (
+      fail g (Some <| head_range t)
+          (Printf.sprintf "check_withlocal: allocating a local variable: type %s is not universe zero (computed %s)"
+              (P.term_to_string init)
+              (P.univ_to_string init_u))
+    )
+    else
+      let x = fresh g in
+      let px = binder.binder_ppname, x in
+      if x `Set.mem` freevars_st body
+      then fail g (Some body.range) (Printf.sprintf "withlocal: %s is free in body" (T.unseal binder.binder_ppname.name))
       else
-        let body_post = extend_post_hint_for_local g post init_t x in
-        let (| opened_body, c_body, body_typing |) =
-          let r =
-            check g_extended body_pre body_pre_typing (Some body_post) binder.binder_ppname (open_st_term_nv body px) in
-          apply_checker_result_k r binder.binder_ppname in
-        //
-        // Checking post equality here to match the typing rule
-        // 
-        if not (C_ST? c_body)
-        then fail g (Some body.range)
-               (Printf.sprintf "check_withlocal: body computation type %s is not ST"
-                  (P.comp_to_string c_body))
+        let x_tm = term_of_nvar px in
+        let g_extended = push_binding g x binder.binder_ppname (mk_ref init_t) in
+        let body_pre = comp_withlocal_body_pre pre init_t x_tm init in
+        let body_pre_typing = with_local_pre_typing pre_typing init_t x init in
+        // elaborating this post here,
+        //   so that later we can check the computed post to be equal to this one
+        let post : post_hint_for_env g = post in
+        if x `Set.mem` freevars post.post
+        then fail g None "Impossible! check_withlocal: unexpected name clash in with_local,\
+                          please file a bug-report"
         else
+          let body_post = extend_post_hint_for_local g post init_t x in
+          let (| opened_body, c_body, body_typing |) =
+            let r =
+              check g_extended body_pre body_pre_typing (Some body_post) binder.binder_ppname (open_st_term_nv body px) in
+            apply_checker_result_k r binder.binder_ppname in
           let body = close_st_term opened_body x in
           assume (open_st_term (close_st_term opened_body x) x == opened_body);
           let c = C_ST {u=comp_u c_body;res=comp_res c_body;pre;post=post.post} in
           let c_typing =
             let post_typing_rec = post_hint_typing g post x in
-            intro_comp_typing g c pre_typing post_typing_rec.ty_typing x post_typing_rec.post_typing
+            intro_comp_typing g c pre_typing 
+              post_typing_rec.effect_annot_typing 
+              post_typing_rec.ty_typing
+              x post_typing_rec.post_typing
           in
           let d = T_WithLocal g binder.binder_ppname init body init_t c x
             init_typing
@@ -119,8 +131,3 @@ let check
             c_typing
             body_typing in
           checker_result_for_st_typing (| _, _, d |) res_ppname
-
-  else fail g (Some t.range)
-         (Printf.sprintf "check_withlocal: allocating a local variable: type %s is not universe zero (computed %s)"
-            (P.term_to_string init)
-            (P.univ_to_string init_u))
