pulse/lib/steel/pulse/Pulse.Checker.WithLocalArray.fst
@@ -33,7 +33,8 @@ let extend_post_hint
 : T.Tac (q:post_hint_for_env (push_binding g x ppname_default (mk_array init_t)) {
           q.post == comp_withlocal_array_body_post p.post init_t (null_var x) /\
           q.ret_ty == p.ret_ty /\
-          q.u == p.u
+          q.u == p.u /\
+          q.effect_annot == p.effect_annot
         })
 = let arr = null_var x in
   let conjunct = (tm_exists_sl u0 (as_binder (mk_seq u0 init_t)) (mk_array_pts_to init_t arr (null_bvar 0))) in
@@ -70,6 +71,10 @@ let is_annotated_type_array (t:term) : option term =
   | _ -> None
 
 #push-options "--z3rlimit_factor 4 --fuel 0 --ifuel 1"
+let head_range (t:st_term {Tm_WithLocalArray? t.term}) : range =
+  let Tm_WithLocalArray { initializer } = t.term in
+  initializer.range
+
 let check
   (g:env)
   (pre:term)
@@ -78,77 +83,85 @@ let check
   (res_ppname:ppname)
   (t:st_term { Tm_WithLocalArray? t.term })
   (check:check_t)
-  : T.Tac (checker_result_t g pre post_hint) =
+: T.Tac (checker_result_t g pre post_hint)
+= match post_hint with
+  | None ->
+    fail g (Some <| head_range t)
+      "Allocating a mutable local variable expects an annotated post-condition"
 
-  let g = push_context "check_withlocal_array" t.range g in
-  let Tm_WithLocalArray {binder; initializer; length; body} = t.term in
-  let (| init, init_u, init_t, init_t_typing, init_typing |) =
-    (* Check against annotation if any *)
-    let ty = binder.binder_ty in
-    match ty.t with
-    | Tm_Unknown -> compute_tot_term_type_and_u g initializer
-    | _ ->
-      match is_annotated_type_array ty with
-      | None ->
-        fail g (Some ty.range)
-          (Printf.sprintf "expected annotated type to be an array, found: %s"
-             (P.term_to_string ty))
-      | Some ty ->
-        let (| u, ty_typing |) = check_universe g ty in
-        let (| init, init_typing |) =
-          check_term g initializer T.E_Total ty in
-        let ty_typing : universe_of g ty u = ty_typing in
-        let init_typing : typing g init T.E_Total ty = init_typing in
-        (| init, u, ty, ty_typing, init_typing |)
-        <: (t:term & u:universe & ty:term & universe_of g ty u & tot_typing g t ty)
-        (* ^ Need this annotation *)
-  in
-  let (| len, len_typing |) =
-    check_tot_term g length tm_szt in
-  if eq_univ init_u u0
-  then
-    let x = fresh g in
-    let px = binder.binder_ppname, x in
-    if x `Set.mem` freevars_st body
-    then fail g
-              (Some body.range)
-              (Printf.sprintf "withlocalarray: %s is free in body"
-                 (T.unseal binder.binder_ppname.name))
-    else
-      let x_tm = term_of_nvar px in
-      let g_extended = push_binding g x binder.binder_ppname (mk_array init_t) in
-      let body_pre = comp_withlocal_array_body_pre pre init_t x_tm init len in
-      let body_pre_typing =
-        with_local_array_pre_typing pre_typing init_t init len init_typing len_typing x in
-      // elaborating this post here,
-      //   so that later we can check the computed post to be equal to this one
-      let post : post_hint_for_env g =
-        match post_hint with
-        | Some post -> post
+  | Some { effect_annot = EffectAnnotGhost }
+  | Some { effect_annot = EffectAnnotAtomic _ } ->
+    fail g (Some <| head_range t)
+      "Allocating a mutable local variable is only allowed in non-ghost and non-atomic code"
+  
+  | Some post ->
+    let g = push_context "check_withlocal_array" t.range g in
+    let Tm_WithLocalArray {binder; initializer; length; body} = t.term in
+    let (| init, init_u, init_t, init_t_typing, init_typing |) =
+      (* Check against annotation if any *)
+      let ty = binder.binder_ty in
+      match ty.t with
+      | Tm_Unknown -> compute_tot_term_type_and_u g initializer
+      | _ ->
+        match is_annotated_type_array ty with
         | None ->
-          fail g None "Allocating a mutable local array expects an annotated post-condition"
-      in
-      if x `Set.mem` freevars post.post
-      then fail g None "Impossible! check_withlocal: unexpected name clash in with_local,\
-                        please file a bug-report"
+          fail g (Some ty.range)
+            (Printf.sprintf "expected annotated type to be an array, found: %s"
+              (P.term_to_string ty))
+        | Some ty ->
+          let (| u, ty_typing |) = check_universe g ty in
+          let (| init, init_typing |) =
+            check_term g initializer T.E_Total ty in
+          let ty_typing : universe_of g ty u = ty_typing in
+          let init_typing : typing g init T.E_Total ty = init_typing in
+          (| init, u, ty, ty_typing, init_typing |)
+          <: (t:term & u:universe & ty:term & universe_of g ty u & tot_typing g t ty)
+          (* ^ Need this annotation *)
+    in
+    let (| len, len_typing |) =
+      check_tot_term g length tm_szt in
+    if not (eq_univ init_u u0)
+    then (
+      fail g (Some <| head_range t)
+             (Printf.sprintf "check_withlocalarray: allocating a local variable: type %s is not universe zero (computed %s)"
+                (P.term_to_string init)
+                (P.univ_to_string init_u))
+    )
+    else
+      let x = fresh g in
+      let px = binder.binder_ppname, x in
+      if x `Set.mem` freevars_st body
+      then fail g
+                (Some body.range)
+                (Printf.sprintf "withlocalarray: %s is free in body"
+                  (T.unseal binder.binder_ppname.name))
       else
-        let body_post = extend_post_hint g post init_t x in
-        let (| opened_body, c_body, body_typing |) =
-          let r =
-            check g_extended body_pre body_pre_typing (Some body_post) binder.binder_ppname (open_st_term_nv body px) in
-          apply_checker_result_k r binder.binder_ppname in
-
-        if not (C_ST? c_body)
-        then fail g (Some body.range)
-               (Printf.sprintf "check_withlocalarray: body computation type %s is not ST"
-                  (P.comp_to_string c_body))
+        let x_tm = term_of_nvar px in
+        let g_extended = push_binding g x binder.binder_ppname (mk_array init_t) in
+        let body_pre = comp_withlocal_array_body_pre pre init_t x_tm init len in
+        let body_pre_typing =
+          with_local_array_pre_typing pre_typing init_t init len init_typing len_typing x in
+        // elaborating this post here,
+        //   so that later we can check the computed post to be equal to this one
+        let post : post_hint_for_env g = post in
+        if x `Set.mem` freevars post.post
+        then fail g None "Impossible! check_withlocal: unexpected name clash in with_local,\
+                          please file a bug-report"
         else
+          let body_post = extend_post_hint g post init_t x in
+          let (| opened_body, c_body, body_typing |) =
+            let r =
+              check g_extended body_pre body_pre_typing (Some body_post) binder.binder_ppname (open_st_term_nv body px) in
+            apply_checker_result_k r binder.binder_ppname in
           let body = close_st_term opened_body x in
           assume (open_st_term (close_st_term opened_body x) x == opened_body);
           let c = C_ST {u=comp_u c_body;res=comp_res c_body;pre;post=post.post} in
           let c_typing =
             let post_typing_rec = post_hint_typing g post x in
-            intro_comp_typing g c pre_typing post_typing_rec.ty_typing x post_typing_rec.post_typing
+            intro_comp_typing g c pre_typing 
+              post_typing_rec.effect_annot_typing
+              post_typing_rec.ty_typing
+              x post_typing_rec.post_typing
           in
           let d = T_WithLocalArray g binder.binder_ppname init len body init_t c x
             init_typing
@@ -157,8 +170,3 @@ let check
             c_typing
             body_typing in
           checker_result_for_st_typing (| _, _, d |) res_ppname
-
-  else fail g (Some t.range)
-         (Printf.sprintf "check_withlocalarray: allocating a local variable: type %s is not universe zero (computed %s)"
-            (P.term_to_string init)
-            (P.univ_to_string init_u))
