pulse/lib/steel/pulse/Pulse.JoinComp.fst
@@ -76,106 +76,7 @@ let lift_ghost_to_atomic
 (* This matches the effects of the two branches, without
 necessarily matching inames. *)
 #push-options "--z3rlimit 20"
-let join_comp_effects
-  (g_then:env)
-  (e_then:st_term)
-  (c_then:comp_st)
-  (e_then_typing:st_typing g_then e_then c_then)
-  (g_else:env)
-  (e_else:st_term)
-  (c_else:comp_st)
-  (e_else_typing:st_typing g_else e_else c_else)
-  : TacS (c_then':comp_st &
-          c_else':comp_st &
-          st_typing g_then e_then c_then' &
-          st_typing g_else e_else c_else')
-         (requires True) // comp_pre c_then == comp_pre c_else)
-         (ensures fun (| c_then', c_else', _, _ |) ->
-            st_comp_of_comp c_then' == st_comp_of_comp c_then /\
-            st_comp_of_comp c_else' == st_comp_of_comp c_else /\
-            ctag_of_comp_st c_then' == ctag_of_comp_st c_else')
-= let g = g_then in
-  match c_then, c_else with
-  | C_STGhost _, C_STGhost _ 
-  | C_STAtomic _ _ _, C_STAtomic _ _ _
-  | C_ST _, C_ST _ ->
-    (* Nothing to do *)
-    (| c_then, c_else, e_then_typing, e_else_typing |)
-
-  | C_STAtomic _ _ _ , C_ST _ ->
-    let (| c_then', e_then_typing' |) = lift_atomic_to_st g_then e_then c_then e_then_typing in
-    (| c_then', c_else, e_then_typing', e_else_typing |)
-
-  | C_ST _, C_STAtomic _ _ _ ->
-    let (| c_else', e_else_typing' |) = lift_atomic_to_st g_else e_else c_else e_else_typing in
-    (| c_then, c_else', e_then_typing, e_else_typing' |)
-
-  | C_STGhost _, C_STAtomic _ _ _ ->
-    let (| c_then', e_then_typing' |) = lift_ghost_to_atomic g_then e_then c_then e_then_typing in
-    (| c_then', c_else, e_then_typing', e_else_typing |)
-
-  | C_STAtomic _ _ _, C_STGhost _ ->
-    let (| c_else', e_else_typing' |) = lift_ghost_to_atomic g_else e_else c_else e_else_typing in
-    (| c_then, c_else', e_then_typing, e_else_typing' |)
-
-  | C_STGhost _, C_ST _ ->
-    let (| c_then', e_then_typing' |) = lift_ghost_to_atomic g_then e_then c_then  e_then_typing  in
-    let (| c_then', e_then_typing' |) = lift_atomic_to_st    g_then e_then c_then' e_then_typing' in
-    (| c_then', c_else, e_then_typing', e_else_typing |)
-
-  | C_ST _, C_STGhost _ ->
-    let (| c_else', e_else_typing' |) = lift_ghost_to_atomic g_else e_else c_else  e_else_typing  in
-    let (| c_else', e_else_typing' |) = lift_atomic_to_st    g_else e_else c_else' e_else_typing' in
-    (| c_then, c_else', e_then_typing, e_else_typing' |)
-#pop-options
-
-(* Takes the two branches, with already matched effect,
-and matches their invariants (unless C_ST) *)
-#push-options "--z3rlimit 20"
-let join_comp_inames
-  (g_then:env)
-  (e_then:st_term)
-  (c_then:comp_st)
-  (e_then_typing:st_typing g_then e_then c_then)
-  (g_else:env)
-  (e_else:st_term)
-  (c_else:comp_st)
-  (e_else_typing:st_typing g_else e_else c_else)
-  : TacS (c_then':comp_st &
-          c_else':comp_st &
-          st_typing g_then e_then c_then' &
-          st_typing g_else e_else c_else')
-         (requires ctag_of_comp_st c_then == ctag_of_comp_st c_else)
-         (ensures fun (| c_then', c_else', _, _ |) ->
-            st_comp_of_comp c_then' == st_comp_of_comp c_then /\
-            st_comp_of_comp c_else' == st_comp_of_comp c_else /\
-            ctag_of_comp_st c_then' == ctag_of_comp_st c_then /\
-            ctag_of_comp_st c_else' == ctag_of_comp_st c_else /\
-            inames_of_comp c_then' == inames_of_comp c_else' /\
-            obs_of_comp c_then' == obs_of_comp c_else'
-         )
-= match c_then, c_else with
-  | C_ST _, C_ST _
-  | C_STGhost _, C_STGhost _ ->
-    (| c_then, c_else, e_then_typing, e_else_typing |)
-
-  | C_STAtomic inames1 obs1 stc_then, C_STAtomic inames2 obs2 stc_else ->
-    if eq_tm inames1 inames2 && obs1 = obs2 then
-      (* easy case; an optimization *)
-      (| c_then, c_else, e_then_typing, e_else_typing |)
-    else (
-      let is = compute_iname_join inames1 inames2 in
-      // FIXME: this should come from some meta-theorem, we always have is1 `subset` join is1 is2
-      let tok1 : prop_validity g_then (tm_inames_subset inames1 is) = RU.magic () in
-      let tok2 : prop_validity g_else (tm_inames_subset inames2 is) = RU.magic () in
-      let e_then_typing = T_Sub _ _ _ _ e_then_typing (STS_AtomicInvs g_then stc_then inames1 is obs1 (join_obs obs1 obs2) tok1) in
-      let e_else_typing = T_Sub _ _ _ _ e_else_typing (STS_AtomicInvs g_else stc_else inames2 is obs2 (join_obs obs1 obs2) tok2) in
-      (| C_STAtomic is _ stc_then, C_STAtomic is _ stc_else, e_then_typing, e_else_typing |)
-    )
-
-#pop-options
-
-#push-options "--z3rlimit 20"
+open Pulse.Checker.Base
 (* NB: g_then and g_else are equal except for containing one extra
 hypothesis according to which branch was taken. *)
 let join_comps
@@ -187,21 +88,25 @@ let join_comps
   (e_else:st_term)
   (c_else:comp_st)
   (e_else_typing:st_typing g_else e_else c_else)
+  (post:post_hint_t)
   : TacS (c:comp_st &
           st_typing g_then e_then c &
           st_typing g_else e_else c)
-         (requires comp_pre c_then == comp_pre c_else)
-         (ensures fun (| c, _, _ |) -> st_comp_of_comp c == st_comp_of_comp c_then)
-=
-  let g = g_then in
-  if not (eq_st_comp (st_comp_of_comp c_then) (st_comp_of_comp c_else)) then
-    fail g None "Cannot combine then and else branches (different st_comp)";
-
-  let (| c_then', c_else', e_then_typing', e_else_typing' |) =
-    join_comp_effects g_then e_then c_then e_then_typing g_else e_else c_else e_else_typing in
-  assert (ctag_of_comp_st c_then' == ctag_of_comp_st c_else');
-  let (| c_then'', c_else'', e_then_typing'', e_else_typing'' |) =
-    join_comp_inames g_then e_then c_then' e_then_typing' g_else e_else c_else' e_else_typing' in
-  assert (c_then'' == c_else'');
-  (| c_then'', e_then_typing'', e_else_typing'' |)
+         (requires
+            comp_post_matches_hint c_then (Some post) /\
+            comp_post_matches_hint c_else (Some post) /\
+            comp_pre c_then == comp_pre c_else)
+         (ensures fun (| c, _, _ |) ->
+           st_comp_of_comp c == st_comp_of_comp c_then /\
+           comp_post_matches_hint c (Some post))
+= let g = g_then in
+  assert (st_comp_of_comp c_then == st_comp_of_comp c_else);
+  match c_then, c_else with
+  | C_STAtomic _ obs1 _, C_STAtomic _ obs2 _ ->
+    let obs = join_obs obs1 obs2 in
+    let e_then_typing = T_Lift _ _ _ _ e_then_typing (Lift_Observability g_then c_then obs) in
+    let e_else_typing = T_Lift _ _ _ _ e_else_typing (Lift_Observability g_else c_else obs) in
+    (| _, e_then_typing, e_else_typing |)
+  | _ -> 
+    (| _, e_then_typing, e_else_typing |)
 #pop-options
