pulse/lib/steel/pulse/Pulse.JoinComp.fsti
@@ -19,95 +19,12 @@ module Pulse.JoinComp
 open Pulse.Syntax
 open Pulse.Typing
 
-let inames_of_comp (c:comp_st) : term =
-  match c with
-  | C_ST _
-  | C_STGhost _ -> tm_emp_inames
-  | C_STAtomic inames _ _ -> inames
-
-let obs_of_comp (c:comp_st) : observability =
-  match c with
-  | C_ST _ -> Observable
-  | C_STGhost _ -> Neutral
-  | C_STAtomic _ obs _ -> obs
-
-val compute_iname_join (is1 is2 : term) : term
-  
 effect TacS (a:Type) (pre : Type0) (post : (_:a{pre}) -> Type0) =
   Tactics.TacH a (requires (fun _ -> pre))
                  (ensures (fun _ r -> pre /\ (
                                       match r with
                                       | Tactics.Result.Success r _ -> post r
                                       | _ -> True))) // does not guarantee anything on failure
-
-val lift_atomic_to_st
-  (g : env)
-  (e : st_term)
-  (c : comp_st{C_STAtomic? c})
-  (d : st_typing g e c)
-  : Pure (c':comp_st & st_typing g e c')
-         (requires True)
-         (ensures fun (| c', _ |) ->
-             st_comp_of_comp c' == st_comp_of_comp c /\
-             ctag_of_comp_st c' == STT)
-
-val lift_ghost_to_atomic
-  (g : env)
-  (e : st_term)
-  (c : comp_st{C_STGhost? c})
-  (d : st_typing g e c)
-  : TacS (c':comp_st & st_typing g e c')
-         (requires True)
-         (ensures fun (| c', _ |) ->
-             st_comp_of_comp c' == st_comp_of_comp c /\
-             ctag_of_comp_st c' == STT_Atomic /\
-             tm_emp_inames == C_STAtomic?.inames c')
-
-(* This matches the effects of the two branches, without
-necessarily matching inames. *)
-val join_comp_effects
-  (g_then:env)
-  (e_then:st_term)
-  (c_then:comp_st)
-  (e_then_typing:st_typing g_then e_then c_then)
-  (g_else:env)
-  (e_else:st_term)
-  (c_else:comp_st)
-  (e_else_typing:st_typing g_else e_else c_else)
-  : TacS (c_then':comp_st &
-          c_else':comp_st &
-          st_typing g_then e_then c_then' &
-          st_typing g_else e_else c_else')
-         (requires True) // comp_pre c_then == comp_pre c_else)
-         (ensures fun (| c_then', c_else', _, _ |) ->
-            st_comp_of_comp c_then' == st_comp_of_comp c_then /\
-            st_comp_of_comp c_else' == st_comp_of_comp c_else /\
-            ctag_of_comp_st c_then' == ctag_of_comp_st c_else')
-
-(* Takes the two branches, with already matched effect,
-and matches their invariants (unless C_ST) *)
-val join_comp_inames
-  (g_then:env)
-  (e_then:st_term)
-  (c_then:comp_st)
-  (e_then_typing:st_typing g_then e_then c_then)
-  (g_else:env)
-  (e_else:st_term)
-  (c_else:comp_st)
-  (e_else_typing:st_typing g_else e_else c_else)
-  : TacS (c_then':comp_st &
-          c_else':comp_st &
-          st_typing g_then e_then c_then' &
-          st_typing g_else e_else c_else')
-         (requires ctag_of_comp_st c_then == ctag_of_comp_st c_else)
-         (ensures fun (| c_then', c_else', _, _ |) ->
-            st_comp_of_comp c_then' == st_comp_of_comp c_then /\
-            st_comp_of_comp c_else' == st_comp_of_comp c_else /\
-            ctag_of_comp_st c_then' == ctag_of_comp_st c_then /\
-            ctag_of_comp_st c_else' == ctag_of_comp_st c_else /\
-            inames_of_comp c_then' == inames_of_comp c_else' /\
-            obs_of_comp c_then' == obs_of_comp c_else'
-         )
 
 val join_comps
   (g_then:env)
@@ -118,8 +35,14 @@ val join_comps
   (e_else:st_term)
   (c_else:comp_st)
   (e_else_typing:st_typing g_else e_else c_else)
-  : TacS (c:comp_st &
-          st_typing g_then e_then c &
-          st_typing g_else e_else c)
-         (requires comp_pre c_then == comp_pre c_else)
-         (ensures fun (| c, _, _ |) -> st_comp_of_comp c == st_comp_of_comp c_then)
+  (post:post_hint_t)
+: TacS (c:comp_st &
+        st_typing g_then e_then c &
+        st_typing g_else e_else c)
+    (requires
+      comp_post_matches_hint c_then (Some post) /\
+      comp_post_matches_hint c_else (Some post) /\
+      comp_pre c_then == comp_pre c_else)
+    (ensures fun (| c, _, _ |) ->
+        st_comp_of_comp c == st_comp_of_comp c_then /\
+        comp_post_matches_hint c (Some post))
