pulse/lib/steel/pulse/Pulse.Reflection.Util.fst
@@ -156,6 +156,7 @@ let mk_stt_ghost_admit (u:R.universe) (t pre post:R.term) : R.term =
 
 let emp_inames_lid = mk_pulse_lib_core_lid "emp_inames"
 let add_inv_lid = mk_pulse_lib_core_lid "add_inv"
+let remove_inv_lid = mk_pulse_lib_core_lid "remove_inv"
 let elim_pure_lid = mk_pulse_lib_core_lid "elim_pure"
 
  //the thunked, value-type counterpart of the effect STT
@@ -292,6 +293,10 @@ let emp_inames_tm : R.term = R.pack_ln (R.Tv_FVar (R.pack_fv emp_inames_lid))
 
 let add_inv_tm (p is i : R.term) : R.term =
   let h = R.pack_ln (R.Tv_FVar (R.pack_fv add_inv_lid)) in
+  R.mk_app h [im p; ex is; ex i]
+
+let remove_inv_tm (p is i : R.term) : R.term =
+  let h = R.pack_ln (R.Tv_FVar (R.pack_fv remove_inv_lid)) in
   R.mk_app h [im p; ex is; ex i]
 
 let non_informative_witness_lid = mk_pulse_lib_core_lid "non_informative_witness"
